assignments/chapter02/exercise01.dfy
@@ -7,7 +7,10 @@
 ghost predicate IsPrimeSpec(candidate:nat)
 {
   /*{*/
-  false  // Replace me
+  if candidate < 2 then 
+    false
+  else 
+    forall divisor:nat :: 2 <= divisor < candidate ==> (candidate % divisor != 0)
   /*}*/
 }
 
@@ -24,6 +27,12 @@ lemma ConstantObligations()
   ensures !IsPrimeSpec(9)
 {
   /*{*/
+  assert !IsPrimeSpec(0);
+  assert(4%2 == 0);
+  assert(6%2 == 0);
+  assert(9%3 == 0);
+  assert(!IsPrimeSpec(4));
+  assert !IsPrimeSpec(1);
   /*}*/
 }
 
@@ -32,6 +41,7 @@ lemma CompositeIsntPrime(p: nat)
   ensures !IsPrimeSpec(p*66)
 {
   /*{*/
+  assert p*66 % p == 0;
   /*}*/
 }
 
