demos/chapter03/librarycards.dfy
@@ -19,18 +19,46 @@ ghost predicate CheckIn(v:Variables, v':Variables, book:Book, patron:string) {
   && v' == v[book := Shelf]
 }
 
+ghost predicate CheckInVerse(v:Variables, v':Variables, book:Book, patron:string){
+  CheckOut(v', v, book, patron)
+}
+
 ghost predicate Next(v:Variables, v':Variables) {
-  || (exists book, patron :: CheckIn(v, v', book, patron))
+  || (exists book, patron :: CheckInVerse(v, v', book, patron))
   || (exists book, patron :: CheckOut(v, v', book, patron))
 }
 
 ghost predicate Safety(v:Variables) {
-  
+  forall book1, book2 |
+  && book1 in v 
+  && book2 in v 
+  && !v[book1].Shelf?
+  && !v[book2].Shelf? 
+  && v[book1] == v[book2] 
+  :: book1 == book2
 }
 
 lemma SafetyProof()
   ensures forall v | Init(v) :: Safety(v)
   ensures forall v, v' | Safety(v) && Next(v, v') :: Safety(v')
 {
-  
+  forall v:Variables, v':Variables | Safety(v) && Next(v,v') ensures Safety(v') {
+    forall book1, book2 |
+    && book1 in v' 
+    && book2 in v' 
+    && !v'[book1].Shelf?
+    && !v'[book2].Shelf? 
+    && v'[book1] == v'[book2]
+    ensures book1 == book2 
+    // {
+    //   if exists book, patron :: CheckIn(v, v', book, patron){
+    //     assert book1 == book2;
+    //   }
+    //   else if exists book, patron:: CheckOut(v, v', book, patron){
+    //     assert book1 == book2;
+    //   }
+    // }
+    {assert book1 in v;
+    assert book2 in v;} // we need the safety of v for book1 in v' ensures safety of v' but doesnt help in this case
+  }
 }
