assignments/chapter01/exercise19.dfy
@@ -10,6 +10,19 @@ method IsSeqSorted(intSeq:seq<int>) returns (issorted:bool)
     ensures issorted <==> IsSorted(intSeq[..])
 {
   /*{*/
+  var count:nat := 0;
+  if |intSeq| <= 1 {
+    return true;
+  }
+  while (count < |intSeq| -1) 
+  invariant 0 <= count < |intSeq|
+  invariant forall i:nat,j:nat | i<j<=count :: intSeq[i] <= intSeq[j]
+  {
+    if (intSeq[count] > intSeq[count+1]) {
+      return false;
+    }
+    count := count + 1;
+  }
   return true;
   /*}*/
 }
