assignments/chapter01/exercise22.dfy
@@ -24,5 +24,63 @@ method FindInBinaryTree(tree:Tree, needle:int) returns (found:bool)
     ensures found <==> needle in TreeAsSequence(tree)
 {
 /*{*/
+    var found_l := false;
+    var found_r := false;
+    var found_m := false;
+    if tree == Nil {
+        assert needle !in TreeAsSequence(tree);
+        return false;
+    }
+    else if tree.value == needle {
+        // found_m := true;
+        // assert found_m <==> needle in TreeAsSequence(tree);
+        // assert needle in TreeAsSequence(tree) ==> found_m;
+        return true;
+    }
+    else if tree.left == Nil && tree.right == Nil {
+        assert needle !in TreeAsSequence(tree);
+        return false;
+    }
+    // assert !found_m;
+    else if needle < tree.value{
+        if tree.left == Nil {
+            SortedTreeMeansSortedSequence(tree.right);
+            return false;
+        }
+        found_l := FindInBinaryTree(tree.left, needle);
+        assert found_l <==> needle in TreeAsSequence(tree.left);
+        assert SequenceIsSorted(TreeAsSequence(tree.right)) ==> needle !in TreeAsSequence(tree.right);
+        // assert needle < TreeAsSequence(tree.right)[0] && IsSortedTree(tree) <==> !(needle in TreeAsSequence(tree.right));
+        assert tree.value != needle;
+        // assert found_l <==> needle in TreeAsSequence(tree);
+        SortedTreeMeansSortedSequence(tree.right);
+        return found_l;
+    }
+    else if needle > tree.value{
+        if tree.right == Nil {
+            assert SequenceIsSorted(TreeAsSequence(tree.left)) ==> needle !in TreeAsSequence(tree.left);
+            // assert IsSortedTree(tree.left) ==> needle !in TreeAsSequence(tree.left);
+            SortedTreeMeansSortedSequence(tree.left);
+            assert IsSortedTree(tree) ==> SequenceIsSorted(TreeAsSequence(tree));
+            assert SequenceIsSorted(TreeAsSequence(tree.left));
+            assert needle !in TreeAsSequence(tree.left);
+            return false;
+        }
+        found_r := FindInBinaryTree(tree.right, needle);
+        assert found_r <==> needle in TreeAsSequence(tree.right);
+        assert TreeAsSequence(tree) == TreeAsSequence(tree.left) + [tree.value] + TreeAsSequence(tree.right);
+        assert needle in TreeAsSequence(tree.right) ==> needle in TreeAsSequence(tree);
+        assert found_r ==> needle in TreeAsSequence(tree);
+        assert !found_l;
+        assert tree.value != needle;
+        assert tree.left != Nil || tree.right != Nil;
+        SortedTreeMeansSortedSequence(tree.left);
+        // assert (!found_l && found_r && tree.value !=needle) <==> needle in TreeAsSequence(tree);
+        return found_r;
+    }
+
+    // assert found_l || found_r || found_m <==> needle in TreeAsSequence(tree);
+    // return found_l || found_r || found_m;
+
 /*}*/
 }
