assignments/chapter02/exercise03.dfy
@@ -16,11 +16,29 @@ predicate IsSorted(seqint:seq<int>)
 /*}*/
 method merge_sort(input:seq<int>) returns (output:seq<int>)
 /*{*/
-  ensures true  // Replace me
+  ensures IsSorted(output)
+  ensures |output| == |input|
+  decreases |input|
+  ensures multiset(output) == multiset(input)
 /*}*/
 {
 /*{*/
-  // Supply the body.
+  if |input| <= 1 {
+    output := input;
+    return;
+  }
+  var mid := |input| / 2;
+  var left := input[0..mid];
+  var right := input[mid..|input|];
+  var sorted_left := merge_sort(left);
+  var sorted_right := merge_sort(right);
+  assert multiset(sorted_left) == multiset(left);
+  assert multiset(sorted_right) == multiset(right);
+  output := merge(sorted_left, sorted_right);
+  assert multiset(output) == multiset(sorted_left) + multiset(sorted_right);
+  assert input == left + right;
+  assert multiset(input) == multiset(left) + multiset(right);
+  assert multiset(input) == multiset(sorted_left) + multiset(sorted_right);
 /*}*/
 }
 
@@ -28,11 +46,105 @@ method merge(seqa:seq<int>, seqb:seq<int>) returns (output:seq<int>)
   requires IsSorted(seqa)
   requires IsSorted(seqb)
 /*{*/
-  ensures true  // Replace me
+  decreases |seqa| 
+  decreases |seqb|
+  ensures IsSorted(output)
+  ensures |output| == |seqa| + |seqb|
+  ensures multiset(output) == multiset(seqa) + multiset(seqb)
 /*}*/
 {
 /*{*/
-  // Supply the body.
+  var i, j := 0, 0;
+  if |seqa| == 0 {
+    output := seqb;
+    return;
+  }
+  if |seqb| == 0 {
+    output := seqa;
+    return;
+  }
+  output := [];
+  // while i < |seqa| && j < |seqb|
+  //   invariant 0 <= i <= |seqa|
+  //   invariant 0 <= j <= |seqb|
+  //   invariant |output| == i + j
+  //   invariant IsSorted(output)
+  //   invariant i < |seqa| ==> (|output| == 0 || output[|output|-1] <= seqa[i])
+  //   invariant j < |seqb| ==> (|output| == 0 || output[|output|-1] <= seqb[j])
+  //   decreases (|seqa| - i) + (|seqb| - j)
+  //   invariant multiset(output) + multiset(seqa[i..]) + multiset(seqb[j..])
+  //             == multiset(seqa) + multiset(seqb)
+  // {
+  //   if seqa[i] <= seqb[j] {
+  //     output := output + [seqa[i]];
+  //     assert seqa[i] in output;
+  //     assert seqa[i..] == [seqa[i]] + seqa[i+1..];
+  //     i := i + 1;
+  //   } else {
+  //     output := output + [seqb[j]];
+  //     assert seqb[j] in output;
+  //     assert seqb[j..] == [seqb[j]] + seqb[j+1..];
+  //     j := j + 1;
+  //   }
+  // }
+
+  // if j < |seqb| {
+  //   while j < |seqb|
+  //     invariant 0 <= i <= |seqa|
+  //     invariant 0 <= j <= |seqb|
+  //     invariant |output| == i + j
+  //     invariant IsSorted(output)
+  //     invariant IsSorted(seqb)
+  //     invariant j < |seqb| ==> (|output| == 0 || output[|output|-1] <= seqb[j])
+  //     invariant multiset(output) + multiset(seqa[i..]) + multiset(seqb[j..])
+  //               == multiset(seqa) + multiset(seqb)
+  //     decreases |seqb| - j
+  //     {
+  //       output := output + [seqb[j]];
+  //       assert seqb[j..] == [seqb[j]] + seqb[j+1..];
+  //       assert seqb[j] in output;
+  //       j := j + 1;
+  //     }
+  // }
+  
+  // while i < |seqa|
+  //   invariant 0 <= i <= |seqa|
+  //   invariant 0 <= j <= |seqb|
+  //   invariant |output| == i + j
+  //   invariant IsSorted(output)
+  //   invariant  multiset(output) + multiset(seqa[i..]) + multiset(seqb[j..])
+  //             == multiset(seqa) + multiset(seqb)
+  //   invariant (i < |seqa| && |seqa| > 0)  ==> (|output| == 0 || output[|output|-1] <= seqa[i])
+  //   decreases |seqa| - i
+  // {
+  //   output := output + [seqa[i]];
+  //   assert seqa[i] in output;
+  //   assert seqa[i..] == [seqa[i]] + seqa[i+1..];
+  //   i := i + 1;
+  // }
+  // assert IsSorted(seqb);
+  while i < |seqa| || j < |seqb|
+    invariant 0 <= i <= |seqa|
+    invariant 0 <= j <= |seqb|
+    invariant |output| == i + j
+    invariant IsSorted(output)
+    invariant (i < |seqa| && |output| > 0) ==> output[|output|-1] <= seqa[i]
+    invariant (j < |seqb| && |output| > 0) ==> output[|output|-1] <= seqb[j]
+    invariant  multiset(output) + multiset(seqa[i..]) + multiset(seqb[j..])
+              == multiset(seqa) + multiset(seqb)
+    decreases |seqa| + |seqb| - (i + j)
+{
+    if i < |seqa| && (j >= |seqb| || seqa[i] <= seqb[j]) {
+        output := output + [seqa[i]];
+        assert seqa[i..] == [seqa[i]] + seqa[i+1..];
+        i := i + 1;
+    } else {
+        output := output + [seqb[j]];
+        assert seqb[j..] == [seqb[j]] + seqb[j+1..];
+        j := j + 1;
+    }
+  }
+  
 /*}*/
 }
 
