demos/chapter01/recursion.dfy
@@ -1,8 +1,9 @@
 function Evens(count:int) : (outseq:seq<int>)
   ensures forall idx :: 0<=idx<|outseq| ==> outseq[idx] == 2 * idx
+  ensures |outseq| == count
 {
   if count==0 
   then [] 
   else 
-    Evens(count) + [2 * (count-1)]
+    Evens(count-1) + [2 * (count-1)]
 }
