demos/chapter03/triggers.dfy
@@ -1,0 +1,11 @@
+predicate P(x: int)
+predicate Q(x: int)
+predicate R(x: int)
+// it only learns for forall when there is a trigger
+lemma foo() 
+    requires forall x{:trigger P(x)} :: P(x) && Q(x) && R(x)
+    ensures R(0)
+    {
+        // assert P(0);
+        var x := P(0); // it doesn't have to be true, you just have to mention it
+    }
