labs/lab03/lab03_lab.dfy
@@ -1,0 +1,79 @@
+// Write a state machine spec representing the factory floor and robot.
+datatype Color = Red | Blue
+
+datatype Constants = Constants()
+datatype Variables = Variables(factory_stacks: seq<Stack>, robot_stack: Stack, deliveries: nat)
+
+
+// datatype Disk = Disk(color:Color)
+datatype Stack = Stack(items: seq<Color>)
+datatype Robot = Robot(counter:int, stack:Stack)
+datatype Floor = Floor(stacks: array<Stack>)
+// Define any helper predicates/functions as needed.
+
+ghost predicate StackIsALlColor(stack: Stack, color: Color)
+{
+    forall i: nat | i < |stack.items| :: stack.items[i] == color
+}
+
+ghost predicate StackIsALLSameColor(stack:Stack) 
+{
+    StackIsALlColor(stack, Red) || StackIsALlColor(stack, Blue)
+}
+
+ghost predicate Init(c: Constants, v: Variables)
+{
+    // Fill in here
+    && (forall i: nat | i < |v.factory_stacks| :: (|v.factory_stacks[i].items| == 0 || StackIsALLSameColor(v.factory_stacks[i])))
+    && (|v.robot_stack.items| == 0 || StackIsALLSameColor(v.robot_stack))
+}
+
+ghost predicate PickUp(c: Constants, v: Variables, v': Variables, stack_index: nat)
+{
+    // Fill in here
+    && (stack_index<|v.factory_stacks|)
+    && (|v.factory_stacks[stack_index].items|>0)
+    && (|v.robot_stack.items| == 0 || v.robot_stack.items[0] == v.factory_stacks[stack_index].items[0])
+    && (v'.factory_stacks == v.factory_stacks[stack_index := Stack(v.factory_stacks[stack_index].items[1..])])
+    && (v'.robot_stack == Stack([v.factory_stacks[stack_index].items[0]] + v.robot_stack.items))
+    && (v'.deliveries == v.deliveries)
+}
+
+ghost predicate Drop(c: Constants, v: Variables, v': Variables, stack_index: nat)
+{
+    // Fill in here
+    && (stack_index<|v.factory_stacks|)
+    && (|v.robot_stack.items|>0)
+    && (|v.factory_stacks[stack_index].items| == 0 || v.robot_stack.items[0] == v.factory_stacks[stack_index].items[0])
+}
+
+ghost predicate Deliver(c: Constants, v: Variables, v': Variables)
+{
+    // Fill in here
+    true
+}
+
+// Write out the JNF 
+
+
+
+ghost predicate Next(c: Constants, v: Variables, v': Variables)
+{
+    true
+}
+
+
+
+
+ghost predicate Safety(c: Constants, v: Variables)
+{
+    // Fill in the safety condition.
+    true
+}
+
+// Should prove by itself!
+lemma SafetyProof()
+    ensures forall c, v :: Init(c, v) ==> Safety(c, v)
+    ensures forall c, v, v' :: Safety(c, v) && Next(c, v, v') ==> Safety(c, v')
+{
+}
